To be demonstrated:

$$ (x<0 \land y=2) \Rightarrow A \land A \Rightarrow (x<-2 \land y>0) $$

Because of the transitivity of implication it must therefore hold:

$$ (x<0 \land y=2) \Rightarrow (x<-2 \land y>0) $$

Lemma: $ A \Rightarrow (B \land C) \equiv (A \Rightarrow B) \land (A \Rightarrow C) $

Proof:

$$ A \Rightarrow (B \land C) $$
$$ \neg A \lor (B \land C) $$
$$ (\neg A \lor B) \land (\neg A \lor C) $$
$$ (A \Rightarrow B) \land (A \Rightarrow C) $$

It must therefore hold that $x<0 \Rightarrow x<-2$ and $y=2 \Rightarrow y>0$. The first
is not the case when x=-1.

Therefore, no such A can exist.

\iffalse
x<0Λy=2↦x<-2Λy>0

x<0↦x<-2
y=2↦y>0

a:=x<0
b:=y=2
c:=x<-2
d:=y>0

((aΛb)↦A)Λ(A↦(cΛd))Λ(c↦a)Λ(b↦d)

c↦a (eigener Beweis?)
b↦d (eigener Beweis?)

(aΛb)↦(cΛd)
~a∨~b∨(cΛd)
~a∨((~b∨c)Λ(~b∨d))
(~a∨~b∨c)Λ(~a∨~b∨d)

(~a∨~b∨c)Λ(~a∨~b∨d)Λ(~b∨d)

In Klauselform:
{{~a,~b,c},{~a,~b,d},{~b,d},{~c,a}}
Per pure-literal-rule auf ~b:
{{~c,a}}
Per pure-literal-rule auf ~c:
{}

Deswegen nicht erfüllbar.
\fi
\bye
