$$ A:\equiv true $$
$$ B:\equiv \forall n:true $$
$$ C:\equiv \forall n:true \land \forall m:true $$
$$ D:\equiv \forall n:true \land \forall m:true \land m \geq 0 $$
$$ E:\equiv \forall n:true \land \forall m:true \land m \geq 0 \land p = m $$
$$ F:\equiv \forall n:true \land \forall m:true \land m<0 $$
$$ G:\equiv \forall n:true \land \forall m:true \land m<0 \land p=-m $$
$$ H:\equiv \forall n:true \land \forall m:true \land (p=m \lor p=-m) $$
$$ I:\equiv \forall n:true \land \forall m:true \land (p=m \lor p=-m) \land i=0 $$
$$ J:\equiv \forall n:true \land \forall m:true \land (p=m \lor p=-m) \land i=0 \land x=n $$
$$ K:\equiv \forall n:true \land \forall m:true \land (p=m \lor p=-m) \land i \leq p \land p \geq 0 \land x=n^{i+1} $$
$$ L:\equiv \forall n:true \land \forall m:true \land (p=m \lor p=-m) \land i<p \land p \geq 0 \land x=n^{i+1} $$
$$ M:\equiv \forall n:true \land \forall m:true \land (p=m \lor p=-m) \land i<p \land p \geq 0 \land x=n^{i+2} $$
$$ N:\equiv \forall n:true \land \forall m:true \land (p=m \lor p=-m) \land i \leq p \land p \geq 0 \land x=n^{i+1} $$
$$ O:\equiv \forall n:true \land \forall m:true \land (p=m \lor p=-m) \land i=p \land p \geq 0 \land x=n^{i+1} $$
\bye
