\documentclass{article}

\usepackage{amsmath}

\begin{document}

\section*{2.4}

$$ Z:\equiv a \le b \le c $$
$b=t$:
$$ a \le t \le c $$
$a=b$:
$$ b \le t \le c $$
$t=a$:
$$ b \le a \le c $$
$if(a>b)$:
$$ (a>b \Rightarrow a \le b \le c) \land (\neg a>b \Rightarrow b \le a \le c) $$
$c=t$:
$$ (a>b \Rightarrow a \le b \le t) \land (\neg a>b \Rightarrow b \le a \le t) $$
$b=c$:
$$ (a>c \Rightarrow a \le c \le t) \land (\neg a>c \Rightarrow c \le a \le t) $$
$t=b$:
$$ (a>c \Rightarrow a \le c \le b) \land (\neg a>c \Rightarrow c \le a \le b) $$
$if(b>c)$:
$$ (b>c \Rightarrow ((a>c \Rightarrow a \le c \le b) \land (\neg a>c \Rightarrow c \le a \le b))) \land (\neg b>c \Rightarrow a \le b \le c) $$
$b=t$:
$$ (t>c \Rightarrow ((a>c \Rightarrow a \le c \le t) \land (\neg a>c \Rightarrow c \le a \le t))) \land (\neg t>c \Rightarrow a \le t \le c) $$
$a=b$:
$$ (t>c \Rightarrow ((b>c \Rightarrow b \le c \le t) \land (\neg b>c \Rightarrow c \le b \le t))) \land (\neg t>c \Rightarrow b \le t \le c) $$
$t=a$:
$$ (a>c \Rightarrow ((b>c \Rightarrow b \le c \le a) \land (\neg b>c \Rightarrow c \le b \le a))) \land (\neg a>c \Rightarrow b \le a \le c) $$
$if(a>b)$:
\begin{equation}
	\begin{array}{l}
	(a>b \Rightarrow \\
	(a>c \Rightarrow ((b>c \Rightarrow b \le c \le a) \land (\neg b>c \Rightarrow c \le b \le a))) \land (\neg a>c \Rightarrow b \le a \le c)) \\
	\land \\
	(\neg a>b \Rightarrow \\
	(b>c \Rightarrow ((a>c \Rightarrow a \le c \le b) \land (\neg a>c \Rightarrow c \le a \le b))) \land (\neg b>c \Rightarrow a \le b \le c))
	\end{array}
\end{equation}

\begin{equation}
	\begin{array}{l}
	(\neg a>b \lor ((\neg b>c \lor b\le c \le a) \land (b>c \lor c \le b \le a))) \land (a>c \lor b \le a \le c) \\
	\land \\
	(a>b \lor \neg b>c \lor ((\neg a>c \lor a \le c \le b) \land (a>c \lor c \le a \le b))) \land (b>c \lor a \le b \le c)
	\end{array}
\end{equation}

\end{document}
